rich_raven_lang/trnsl.v
@@ -1,0 +1,105 @@
+From stdpp Require Export binders strings.
+From stdpp Require Import countable.
+From stdpp Require Export namespaces.
+From stdpp Require Import gmap list sets.
+
+From iris Require Import options.
+From iris.algebra Require Import cmra.
+From iris.base_logic.lib Require Export own.
+From iris.base_logic.lib Require Import ghost_map.
+From iris.base_logic.lib Require Import invariants.
+
+From iris.proofmode Require Import tactics.
+From iris.program_logic Require Export weakestpre.
+From iris.program_logic Require Import ectx_lifting.
+
+From raven_iris.simp_raven_lang Require Import lang lifting ghost_state.
+From raven_iris.rich_raven_lang Require Import rrl_lang.
+
+
+(* Context `{!simpLangG Σ}. *)
+
+
+Section MainTranslation.
+    (* Context `{!simpLangG Σ}. *)
+  
+    Program Fixpoint trnsl_atomic_annotation (mask: coPset) (a : AtomicAnnotation) {measure match a.2 with | Closed => 0 | Opened s => length s | Stepped s => length s end} : iProp rrl_lang.Σ :=
+      match a.2 with
+      | Closed => True
+      | Opened [] => False
+      | Stepped [] => False
+      | Opened (inv :: invs) => True ∗ trnsl_atomic_annotation (mask ∪ ↑(inv_namespace_map inv.1)) (a.1, Opened invs)
+  
+      | Stepped (inv :: invs) => True ∗ trnsl_atomic_annotation (mask ∪ ↑(inv_namespace_map inv.1)) (a.1, Stepped invs)
+      end
+      .
+      Next Obligation.
+      intros. simpl; subst filtered_var; rewrite <- Heq_anonymous. simpl; lia.
+      Qed.
+      Next Obligation.
+      intros. simpl; subst filtered_var; rewrite <- Heq_anonymous. simpl; lia.
+      Qed.
+      Next Obligation.
+      intros. simpl. Admitted.
+  
+  
+    Definition inv_set_to_namespace (s : gset inv_name) : coPset :=
+      set_fold (λ inv acc, acc ∪ ↑(inv_namespace_map inv)) ∅ s.
+
+      (* Check Σ. *)
+  
+  
+    (* Definition stack_to_stack_frame (stk : stack) : stack_frame := 
+    . *)
+  
+    Definition trnsl_hoare_triple (stk : stack) (stk_frm : stack_frame) (stk_id: stack_id) (p : l_assertion) (a1 : AtomicAnnotation) (cmd : stmt) (stk' : stack) (stk_frm' : stack_frame) (q : l_assertion) (a2 : AtomicAnnotation) : iProp rrl_lang.Σ :=
+        match (trnsl_stmt cmd stk), (trnsl_assertions p), (trnsl_assertions q) with
+        | Error, _, _ | _, None, _ | _, _, None => True
+        | None', Some p', Some q' => 
+          (p' ∗ trnsl_atomic_annotation (inv_set_to_namespace a1.1) a1) -∗ |={(inv_set_to_namespace a1.1), (inv_set_to_namespace a2.1) }=> (q' ∗ trnsl_atomic_annotation (inv_set_to_namespace a2.1) a2)
+        | Some' s, Some p', Some q' => 
+          (* forall (x : Var), trnsl_expressions (stk)-> *)
+          {{{ p' ∗ stack_own[ stk_id, stk_frm ] }}}  to_rtstmt stk_id s  {{{ RET lang.LitUnit; q' ∗ stack_own[ stk_id, stk_frm' ] }}}
+        end
+    .
+  
+    Theorem rrl_validity stk stk_frm stk_id p a1 cmd stk' stk_frm' q a2 :
+      RavenHoareTriple stk p a1 cmd stk' q a2 ->
+      ⊢ (trnsl_hoare_triple stk stk_frm stk_id p a1 cmd stk' stk_frm' q a2).
+    Proof.
+      intros H.
+      destruct H as [ | | | | | | | | | | | | | | | | ].
+      3: {
+        unfold trnsl_hoare_triple.
+        destruct (trnsl_stmt (FldWr e1 fld e2) stk) eqn:Ht. 2:{done. }
+        - inversion Ht. simpl.
+          destruct (trnsl_ravenExpr_lExpr stk e1); try done.
+          destruct (trnsl_ravenExpr_lExpr stk e2); try done.
+          destruct (trnsl_expressions l); try done.
+          destruct (trnsl_expressions l0); try done.
+        
+        -
+          destruct (trnsl_assertions (LOwn lexpr1 fld old_val)) eqn:HOldV; try done.
+          destruct (trnsl_assertions (LOwn lexpr1 fld new_val)) eqn:HNewV; try done.
+        inversion Ht.
+          destruct (trnsl_ravenExpr_lExpr stk e1) eqn:He1; try done.
+          destruct (trnsl_ravenExpr_lExpr stk e2) eqn:He2; try done.
+          destruct (trnsl_expressions l); try done.
+          destruct (trnsl_expressions l0); try done.
+          inversion H3; subst. simpl. destruct H3.
+  
+          (* iApply wp_heap_wr.
+          iModIntro.
+  
+  
+  
+        destruct (trnsl_val old_val). 2:{ simpl. iIntros "[F _]". iExFalso. iFrame. }
+        iIntros  "[Hl HAtm]". 
+      } *)
+  
+  
+    Admitted.
+    
+  
+  
+  End MainTranslation.
